checkpoint some initial code for postconditions instead of >>rec
reason about exec relations instead of exec_recover

problem 1: existential variables span pre and post conditions, making
unification difficult.  currently we explicitly invoke corr_exists in
the proofs in Array.v.

problem 2: no proof automation for pimpl2 (implication for predicates
on two disks).

src/Hoare.v
@@ -6,59 +6,66 @@ Set Implicit Arguments.
 
 (** ** Hoare triples *)
 
-Definition corr (pre: pred) (prog1 prog2: prog) :=
+Definition nonfail (post: pred2) (m m': mem) out :=
+  post m m' /\ out <> Failed.
+
+Definition corr (pre: pred) (post: pred2) (p: prog) :=
   forall m m' out,
   pre m ->
-  exec_recover m prog1 prog2 m' out ->
-  out = Finished.
+  exec m p m' out ->
+  nonfail post m m' out.
 
-Notation "{{ pre }} p1 >> p2" := (corr pre%pred p1 p2)
-  (at level 0, p1 at level 60, p2 at level 60).
+Notation "{{ pre }} p {{ post }}" := (corr pre%pred post%pred2 p)
+  (at level 70, p at level 60).
 
 Theorem pimpl_ok:
-  forall pre pre' pr rec,
-  {{pre'}} pr >> rec ->
+  forall pre pre' pr post post',
+  {{pre'}} pr {{post'}} ->
   (pre ==> pre') ->
-  {{pre}} pr >> rec.
+  (before pre /\ post' ===> post) ->
+  {{pre}} pr {{post}}.
 Proof.
-  firstorder.
+  unfold corr, nonfail.
+  intros.
+  edestruct H; eauto.
+  split; eauto.
+  apply H1.
+  split; eauto.
 Qed.
 
 Theorem pimpl_ok_cont :
-  forall pre pre' A (k : A -> _) x y rec,
-  {{pre'}} k y >> rec ->
+  forall pre pre' A (k : A -> _) x y post post',
+  {{pre'}} k y {{post'}} ->
   (pre ==> pre') ->
   (pre ==> exists F, F * [[x = y]]) ->
-  {{pre}} k x >> rec.
+  (post' ===> post) ->
+  {{pre}} k x {{post}}.
 Proof.
   unfold corr, pimpl; intros.
   edestruct H1; eauto.
-  eapply sep_star_lift_l in H4; [|instantiate (1:=([x=y])%pred)].
-  unfold lift in H4; rewrite H4 in *; eauto.
+  eapply sep_star_lift_l in H5; [|instantiate (1:=([x=y])%pred)].
+  unfold lift in H5; rewrite H5 in *.
+  edestruct H; eauto.
+  unfold nonfail in *; eauto.
   firstorder.
 Qed.
 
 Theorem pimpl_pre:
-  forall pre pre' pr rec,
-  (pre ==> [{{pre'}} pr >> rec]) ->
+  forall pre pre' pr post,
+  (pre ==> [{{pre'}} pr {{post}}]) ->
   (pre ==> pre') ->
-  {{pre}} pr >> rec.
+  {{pre}} pr {{post}}.
 Proof.
-  firstorder.
-Qed.
-
-Theorem pre_false:
-  forall pre p1 p2,
-  (pre ==> [False]) ->
-  {{ pre }} p1 >> p2.
-Proof.
-  firstorder.
+  unfold corr, pimpl, lift.
+  eauto.
 Qed.
 
 Theorem corr_exists:
-  forall T pre p rec,
-  (forall (a:T), {{ pre a }} p >> rec) ->
-  {{ exists a:T, pre a }} p >> rec.
+  forall T pre p post,
+  (forall (a:T), {{ pre a }} p {{ post }}) ->
+  {{ exists a:T, pre a }} p {{ post }}.
 Proof.
-  firstorder.
+  unfold corr, exis; intros.
+  destruct H0.
+  eauto.
 Qed.
